Finish new iterate model

src/polytime/basic.lean
@@ -136,9 +136,9 @@ by { induction n; simp [function.iterate_succ', *], refl, }
 instance : polycodable ℕ :=
 ⟨complexity_class.some.comp polytime.num_nodes⟩
 
-theorem iterate_safe_aux {n : tree unit → ℕ} {f : tree unit → tree unit → tree unit} {st : tree unit → tree unit}
+theorem iterate_aux {n : tree unit → ℕ} {f : tree unit → tree unit → tree unit} {st : tree unit → tree unit}
   (hn : n ∈ₑ PTIME) (hf : f ∈ₑ PTIME) (hst : st ∈ₑ PTIME)
-  (hf' : polysize_safe f) : (λ x, (f x)^[n x] (st x)) ∈ₑ PTIME :=
+  (hf' : polysize_fun (λ (n : ℕ) (x y : tree unit), (f x)^[n] y)) : (λ x, (f x)^[n x] (st x)) ∈ₑ PTIME :=
 begin
   set F : tree unit → tree unit := λ x, x.left △ (f x.left x.right),
   have hF : tree.polytime F := by { dsimp [F], complexity, },
@@ -148,21 +148,28 @@ begin
   refine ⟨_, tree.polytime.right.comp ((tree.polytime.bounded_rec hF _).comp
     (tree.polytime.pair pn (tree.polytime.pair tree.polytime.id pst))), _⟩,
   swap, { intro x, simp only [encode_unit_tree] at hn hst, simp [hF', hn, hst], },
+  cases hf' with p hp,
+  use polynomial.X + p + 1,
+  rintro (_|⟨⟨⟩, n, xy⟩), { simp, },
+  have : ∀ x y, (F^[n.num_nodes] (x △ y)).num_nodes ≤
+    x.num_nodes + (p.eval $ n.num_nodes + (x.num_nodes + y.num_nodes) + 1) + 1,
+  { intros x y, rw hF', specialize hp (n.num_nodes, x, y), simp [has_uncurry.uncurry, add_assoc] at hp ⊢, refine hp.trans (p.eval_mono _), simp, },
+  rcases xy with (_|⟨⟨⟩, x, y⟩),
+  { simp, cases n.num_nodes with n, { simp, }, refine (this _ _).trans _, simp, },
+  { refine (this _ _).trans _, simp [add_assoc x.num_nodes y.num_nodes 1],
+    mono*, exacts [le_add_right $ le_add_left $ le_self_add, le_self_add], },
+end
+
+theorem iterate_safe_aux {n : tree unit → ℕ} {f : tree unit → tree unit → tree unit} {st : tree unit → tree unit}
+  (hn : n ∈ₑ PTIME) (hf : f ∈ₑ PTIME) (hst : st ∈ₑ PTIME)
+  (hf' : polysize_safe f) : (λ x, (f x)^[n x] (st x)) ∈ₑ PTIME :=
+begin
+  apply iterate_aux hn hf hst,
   use polynomial.X + polynomial.X * hf'.poly,
-  rintro (_|⟨⟨⟩, n, (_|⟨⟨⟩, x, y⟩)⟩), { simp, }, swap,
-  { transitivity x.num_nodes + (y.num_nodes + n.num_nodes * (hf'.poly.eval x.num_nodes)) + 1,
-    { simpa [hF'] using hf'.size_le n.num_nodes x y, }, 
-    { have : hf'.poly.eval x.num_nodes ≤ hf'.poly.eval (n.num_nodes + (x.num_nodes + (y.num_nodes + 2))) := hf'.poly.eval_mono (le_add_left $ le_self_add),
-      { simp [add_assoc],
-        refine (le_add_left $ add_le_add_left (add_le_add_left (le_add_left $ _) _) _), conv_lhs { rw add_comm, },
-        refine add_le_add_left (mul_le_mul' le_self_add this) _,  }, } },
-  { -- TODO: write this (and the one above) well; why doesn't linarith work??
-    dsimp, cases n.num_nodes with n, { simp, },
-    convert_to ((f tree.nil)^[n+1] tree.nil).num_nodes + 1 ≤ _, { simp [F, hF'], },
-    rw nat.succ_le_iff,
-    have := (hf'.size_le (n + 1) tree.nil tree.nil), refine lt_of_le_of_lt this _,
-    rw ← nat.succ_le_iff,
-    simp, rw [nat.succ_eq_one_add, add_assoc], refine le_add_left (add_le_add_left (mul_le_mul' le_self_add (hf'.poly.eval_mono zero_le')) _), }
+  rintros ⟨n, x, y⟩,
+  refine (hf'.size_le n x y).trans _,
+  simp [has_uncurry.uncurry], mono*,
+  exacts [le_add_left le_add_self, le_self_add, le_add_left le_self_add, zero_le', zero_le'],
 end
 
 local attribute [complexity] iterate_safe_aux
@@ -203,23 +210,14 @@ end
 @[complexity] lemma polynomial_eval' (p : polynomial ℕ) {f : α → ℕ} (hf : f ∈ₑ PTIME) :
   polytime.mem (λ x, p.eval (f x)) := (polynomial_eval p).comp hf
 
-
 @[complexity] lemma nat_le : polytime.mem_pred ((≤) : ℕ → ℕ → Prop) :=
 by { complexity using (λ x y, x - y = 0), rw tsub_eq_zero_iff_le, }
 
 @[complexity] lemma nat_lt : polytime.mem_pred ((<) : ℕ → ℕ → Prop) :=
 by { complexity using (λ x y, x ≤ y ∧ ¬(y ≤ x)), rw lt_iff_le_not_le, }
 
-/- We now prove that `it` is unconditionally true. The crucial ingredients are:
-  - We can evaluate polynomials in polynomial time
-  - We can prove `tree.guard_size`, which is the identity on trees
-    whose size is less than `n` but otherwise returns a constant garbage value (`nil`),
-    runs in polynomial time.
-  
-Combining these allows us to iterate a function which automatically exits when it takes too long.
-Thus, even on "bad" inputs, it does not take more than polynomial time.
--/
-
+/- Combining these allows us to iterate a function which automatically exits when it takes too long.
+Thus, even on "bad" inputs, it does not take more than polynomial time. -/
 def tree.guard_size (x : tree unit) (n : ℕ) : tree unit :=
 if x.num_nodes ≤ n then x else tree.nil
 
@@ -232,234 +230,46 @@ by { simp only [tree.guard_size], split_ifs, { assumption, }, exact zero_le', }
 lemma tree.guard_size_pos (x : tree unit) {n} (h : x.num_nodes ≤ n) : x.guard_size n = x :=
 by rwa [tree.guard_size, if_pos]
 
-#exit
-/- Our goal in this section is to show that polynomial iteration runs
-  in polynomial time, subject to constraints on the state size not blowing up.
-  
-  One issue that comes up is that our iteration `tree.polytime.prec` requires the
-  function to run in polynomial time on *all* inputs, whereas in general, iterating
-  some `f : α → α` with preprocessing on `g` should only require that `f` runs in polynomial time on valid encodings
-  of `α` which are in the range of `g`.
-  
-  We therefore extract this property, `it`, which states that we can do iteration when
-  the internal state is `α` and preprocessing is `g`. We will show that in fact `it` is always true. This is
-  because we can always check the size of the current state as we are running, and if it is too big,
-  or if we've taken too many steps, we simply stop and output a garbage value (since the input must not have
-  been valid). But in order to prove this, we will need the ability to do some iteration (e.g. comparing nat's,
-  computing tree sizes). Thus, we have a bit of a chicken-egg problem, which is the purpose of having this definition. -/
-private def it (strict : bool) (α β : Type) [tencodable α] [tencodable β] : Prop :=
-∀ (n : α → tree unit) (f : α → α) (g : β → α) 
-  (hn : n ∈ₑ PTIME) (hf : f ∈ₑ PTIME) (hg : g ∈ₑ PTIME)
-  (H : ∃ p : polynomial ℕ, ∀ x (m ≤ (n x).num_nodes), (strict → x ∈ set.range g) → (encode (f^[m] x)).num_nodes ≤ p.eval (encode x).num_nodes),
-  polytime.mem (λ x, f^[(n (g x)).num_nodes] (g x))
+local attribute [-complexity] iterate_safe_aux
 
-/-- As a first step, we show that all `polycodable` types can be iterated on. 
-  We can do this by explicitly decoding and encoding at each step, so that weird things
-  (which may take longer than polynomial time) do not happen on invalid inputs. -/
-private lemma it_of_polycodable (α : Type) [polycodable α] : it ff α β :=
-begin
-  rintros n f g hn hf hg ⟨p, H⟩,
-  refine (_ : polytime.mem (λ x, f^[(n x).num_nodes] x)).comp hg, clear hg,
-  -- TODO: Extract into definition (maybe?)
-  -- A version of f and n which fail "safely" (i.e. if you input something that
-  --  decodes to `none`, the output is `nil`)
-  set f' : tree unit → tree unit := λ s, (encode $ (decode α s).map f).right,
-  set n' : tree unit → tree unit := λ s, (encode $ (decode α s).map n).right,
-  obtain ⟨pf', pn'⟩ : tree.polytime f' ∧ tree.polytime n' := by { split; dsimp [f', n'], complexity, },
-  have H₁ : ∀ x y, decode α x = some y → (f' x = encode (f y) ∧ n' x = n y),
-  { intros x y h, dsimp [f', n'], simp [h, encode], },
-  have H₂ : ∀ x, decode α x = none → f' x = tree.nil ∧ n' x = tree.nil,
-  { intros x h, dsimp [f', n'], simp [h, encode], },
-  have H₃ : ∀ y, f' (encode y) = encode (f y) ∧ n' (encode y) = n y := λ y, H₁ (encode y) _ (tencodable.encodek _),
-  have H₃i : ∀ y m, f'^[m] (encode y) = encode (f^[m] y),
-  { intros y m, induction m with m ih, { simp, },  simp [function.iterate_succ', ih, (H₃ _).1], },
-  have H₄ : ∀ x y m, decode α x = some y → (f'^[m + 1] x = encode (f^[m + 1] y)),
-  { intros x y m h, simp [H₁ x y h, H₃i], },
-  refine ⟨_, tree.polytime.prec pn' pf' _, _⟩, swap,
-  { intro x, simp [(H₃ x).2, has_uncurry.uncurry, H₃i], },
-  cases polycodable.decode_num_nodes_le α with u hu,
-  refine ⟨polynomial.X + (p.comp u), λ x m hm, _⟩,
-  cases m, { simp, },
-  cases hd : decode α x with y, { exfalso, simpa [H₂ x hd] using hm, },
-  simp only [H₄ _ _ m hd, (H₁ _ _ hd).2, polynomial.eval_add, polynomial.eval_X, polynomial.eval_comp] at ⊢ hm,
-  exact le_add_left ((H _ _ hm bool.not_ff.elim).trans $ p.eval_mono $ hu _ _ hd),
+theorem iterate_encode_size {n : α → ℕ} {f : α → β → β} {g : α → β} : n ∈ₑ PTIME → f ∈ₑ PTIME → g ∈ₑ PTIME → 
+  (∃ p : polynomial ℕ, ∀ x (m ≤ n x), (encode $ (f x)^[m] (g x)).num_nodes ≤ p.eval (encode x).num_nodes) →
+  polytime.mem (λ x, (f x)^[n x] (g x))
+| ⟨n', pn, hn⟩ ⟨f', pf, hf⟩ ⟨g', pg, hg⟩ ⟨p, hp⟩ := begin
+  refine ⟨λ x, (λ y, (f' (x △ y)).guard_size (p.eval $ x.num_nodes))^[(n' x).num_nodes] (g' x), _, _⟩,
+  { rw [complexity_class.prop_iff_mem] at *, apply iterate_aux,
+    { complexity, }, { complexity, }, { exact pg, },
+    use p + polynomial.X,
+    rintros ⟨(_|n), x, y⟩, { simp [has_uncurry.uncurry, ← add_assoc], },
+    transitivity p.eval x.num_nodes,
+    { simpa [-iterate_succ, iterate_succ_apply', has_uncurry.uncurry] using tree.guard_size_num_nodes_le _ _, },
+    simp only [polynomial.eval_add, polynomial.eval_X],
+    exact le_add_right (p.eval_mono $ le_add_left le_self_add), },
+  intros x,
+  dsimp only [has_uncurry.uncurry, id] at hn hf hg ⊢,
+  simp only [prod.forall, encode_prod] at hf,
+  simp only [hn, hg, encode_num_nodes],
+  specialize hp x, revert hp, generalize : (n x) = M, intro hp,
+  induction M with M ih, { simp, },
+  specialize ih (λ m hm, hp m (nat.le_succ_of_le hm)), specialize hp _ rfl.le,
+  simp only [iterate_succ_apply', ih, hf] at ⊢ hp,
+  rwa tree.guard_size_pos,
 end
 
-variables [polysize α] [polysize β] {strict : bool}
-
-/-- Similar to the basic `it` property, but we use `size` instead of `(encode x).num_nodes` -/
-private lemma it₁ (hiter : it strict α β) 
-  (n : α → tree unit) (f : α → α) (g : β → α) 
-  (hn : n ∈ₑ PTIME) (hf : f ∈ₑ PTIME) (hg : g ∈ₑ PTIME)
-  (H : ∃ p : polynomial ℕ, ∀ x (m ≤ (n x).num_nodes), (strict → x ∈ set.range g) → size (f^[m] x) ≤ p.eval (size x)) :
-  polytime.mem (λ x, f^[(n (g x)).num_nodes] (g x)) :=
-begin
-  apply hiter n f g hn hf hg,
-  obtain ⟨⟨l, hl⟩, ⟨u, hu⟩, ⟨p, hp⟩⟩ := ⟨polysize.lower α, polysize.upper α, H⟩,
-  refine ⟨l.comp (p.comp u), λ x m h hs, _⟩,
-  simp only [polynomial.eval_comp],
-  exact (hl _).trans (l.eval_mono $ (hp _ _ h hs).trans $ p.eval_mono $ hu _),
-end
-
-private lemma it₂ (hiter : it strict (α × β) α) {n : α → tree unit} {f : α → β → β} {g : α → β} (hn : n ∈ₑ polytime)
-  (hf : f ∈ₑ polytime) (hg : g ∈ₑ polytime)
-  (hp : ∃ p : mv_polynomial (fin 2) ℕ, ∀ x (m ≤ (n x).num_nodes), ∀ y, (strict → y = g x) → size ((f x)^[m] y) ≤ mv_polynomial.eval ![size x, size y] p) :
-  polytime.mem (λ x, (f x)^[(n x).num_nodes] (g x)) :=
-begin
-  set f' := λ xy : α × β, (xy.1, f xy.1 xy.2),
-  have hf' : ∀ n x y, f'^[n] (x, y) = (x, (f x)^[n] y),
-  { intros n x y, induction n with n ih generalizing y, { simp, }, { simp [ih], } }, 
-  have := it₁ hiter (λ xy, n (prod.fst xy)) f' (λ x, (x, g x)) (by complexity) (by complexity) (by complexity) _,
-  { convert complexity_class.mem.snd.comp this, ext x, simp [hf'], },
-  cases hp with p hp,
-  use (mv_polynomial.X 0 + p).to_polynomial,
-  rintros ⟨x₁, x₂⟩ m hm hs,
-  simp at hm hs ⊢,
-  refine trans _ (mv_polynomial.le_to_polynomial_of_le_sum₂ _ _ _),
-  simpa [hf'] using hp x₁ m hm x₂ (λ H, (hs H).symm),
-end
-
-/-- The same as `it₂` but `n` is a function to `ℕ` now -/
-private theorem it₃ (hiter : it strict (α × β) α) {n : α → ℕ} {f : α → β → β} {g : α → β} (hn : n ∈ₑ PTIME)
-  (hf : f ∈ₑ PTIME) (hg : g ∈ₑ PTIME) 
-  (hp : ∃ p : mv_polynomial (fin 2) ℕ, ∀ x (m ≤ n x) y, (strict → y = g x) → size ((f x)^[m] y) ≤ mv_polynomial.eval ![size x, size y] p) :
-  polytime.mem (λ x, (f x)^[n x] (g x)) :=
-by have := it₂ hiter (complexity_class.encode.comp hn) hf hg _; simpa
-
-/-- The condition on `f` is a "local" condition, rather than one involving the iteration of `f` -/
-private lemma it₄ (hiter : it strict (α × β) α) {n : α → ℕ}
-  {f : α → β → β} {g : α → β} (hn : n ∈ₑ PTIME) (hf : f ∈ₑ PTIME) (hg : g ∈ₑ PTIME) 
-  (hp : polysize_safe f) : polytime.mem (λ x, (f x)^[n x] (g x)) :=
-let ⟨p, H⟩ := hp.iterate (polytime.size_le hn) in
-  it₃ hiter hn hf hg ⟨p, λ x m hm y _, H x y m hm⟩
-
-/-- We extract `it₄` on the case of polycodable states so that we can mark
-  it to be used by automation in this section. -/
-theorem iterate_safe' {α β : Type} [polycodable α] [polycodable β] [polysize α] [polysize β]
-  {n : α → ℕ} {f : α → β → β} {g : α → β} (hn : n ∈ₑ PTIME) (hf : f ∈ₑ PTIME) (hg : g ∈ₑ PTIME) 
-  (hp : polysize_safe f) : polytime.mem (λ x, (f x)^[n x] (g x)) :=
-it₄ (it_of_polycodable (α × β)) hn hf hg hp
-
-local attribute [complexity] iterate_safe'
-
-lemma nil_node_iterate (n : ℕ) (y : tree unit) : ((λ x, tree.nil △ x)^[n] y).num_nodes = y.num_nodes + n :=
-by { induction n; simp [function.iterate_succ', *], refl, }
-
-/-- We can measure the number of nodes by iterating `nil △` `x.num_nodes` times -/
-@[complexity] lemma num_nodes : (@tree.num_nodes unit) ∈ₑ PTIME :=
-⟨λ x, (λ y : tree unit, tree.nil △ y)^[x.num_nodes] tree.nil, 
-begin
-  rw [complexity_class.prop_iff_mem],
-  apply it₂ (it_of_polycodable (tree unit × tree unit)), complexity,
-  use mv_polynomial.X 1 + mv_polynomial.X 0,
-  intros x m hm y _,
-  simpa [nil_node_iterate] using hm,
-end, λ x, by { rw [← encode_nat_eq_iterate], refl, }⟩
-
-instance : polycodable ℕ :=
-⟨complexity_class.some.comp polytime.num_nodes⟩
-
-/- Thus, we have that `ℕ` is `polycodable` so we can iterate on `ℕ`.
-  We may therefore prove basic functions (`+`, `*`, `≤`) are polytime.
-  Note that `ℕ` is encoded in a unary fashion here.  -/
-
-@[complexity] lemma add : polytime.mem ((+) : ℕ → ℕ → ℕ) :=
-by { complexity using (λ x y, nat.succ^[y] x), { use 1, simp, }, simp [nat.succ_iterate], }
-
-@[complexity] lemma mul : polytime.mem ((*) : ℕ → ℕ → ℕ) :=
-begin
-  complexity using (λ x y, (+x)^[y] 0),
-  induction y; simp [iterate_succ', nat.mul_succ, *, mul_comm],
-end
-
-/-- For any fixed polynomial `p`, `p.eval` runs in polynomial time -/
-lemma polynomial_eval (p : polynomial ℕ) :
-  polytime.mem (λ n : ℕ, p.eval n) :=
-begin
-  induction p using polynomial.induction_on with p p q ih₁ ih₂ p q ih,
-  { simpa using polytime.const _, },
-  { simpa using add.comp₂ ih₁ ih₂, },
-  simpa [pow_add, ← mul_assoc] using mul.comp₂ ih polytime.id',
-end
-
-@[complexity] lemma polynomial_eval' (p : polynomial ℕ) {f : α → ℕ} (hf : f ∈ₑ PTIME) :
-  polytime.mem (λ x, p.eval (f x)) := (polynomial_eval p).comp hf
-
-@[complexity] lemma tsub : (@has_sub.sub ℕ _) ∈ₑ PTIME :=
-by { complexity using (λ x y, nat.pred^[y] x), { use 0, simpa using nat.pred_le, }, rw nat.pred_iterate, }
-
-@[complexity] lemma nat_le : polytime.mem_pred ((≤) : ℕ → ℕ → Prop) :=
-by { complexity using (λ x y, x - y = 0), rw tsub_eq_zero_iff_le, }
-
-lemma nat_lt : polytime.mem_pred ((<) : ℕ → ℕ → Prop) :=
-by { complexity using (λ x y, x ≤ y ∧ ¬(y ≤ x)), rw lt_iff_le_not_le, }
-
-/- We now prove that `it` is unconditionally true. The crucial ingredients are:
-  - We can evaluate polynomials in polynomial time
-  - We can prove `tree.guard_size`, which is the identity on trees
-    whose size is less than `n` but otherwise returns a constant garbage value (`nil`),
-    runs in polynomial time.
-  
-Combining these allows us to iterate a function which automatically exits when it takes too long.
-Thus, even on "bad" inputs, it does not take more than polynomial time.
--/
-
-def tree.guard_size (x : tree unit) (n : ℕ) : tree unit :=
-if x.num_nodes ≤ n then x else tree.nil
-
-@[complexity] lemma tree_guard_size : tree.guard_size ∈ₑ PTIME :=
-by { delta tree.guard_size, complexity, }
-
-lemma tree.guard_size_num_nodes_le (x : tree unit) (n) : (x.guard_size n).num_nodes ≤ n :=
-by { simp only [tree.guard_size], split_ifs, { assumption, }, exact zero_le', }
-
-lemma tree.guard_size_pos (x : tree unit) {n} (h : x.num_nodes ≤ n) : x.guard_size n = x :=
-by rwa [tree.guard_size, if_pos]
-
-private lemma it_all (α β : Type) [tencodable α] [tencodable β] : it tt α β :=
-begin
-  rintros n f g ⟨n', pn, hn⟩ ⟨f', pf, hf⟩ ⟨g', pg, hg⟩ ⟨p, H⟩,
-  refine ⟨λ x, (λ s : tree unit, (f' s).guard_size (p.eval (g' x).num_nodes))^[(n' (g' x)).num_nodes] (g' x), _, λ x, _⟩,
-  { rw [complexity_class.prop_iff_mem] at *, apply it₃ (it_of_polycodable (tree unit × tree unit)), 
-    complexity,
-    cases size_le pg with pg' hpg',
-    use (mv_polynomial.X 1 + polynomial.to_mv 0 (p.comp pg')),
-    intros x m _ y _, 
-    cases m, { simp, },
-    rw iterate_succ_apply',
-    simpa using le_add_left ((tree.guard_size_num_nodes_le _ _).trans $ p.eval_mono $ hpg' x), },
-  rw [hg, hn],
-  dsimp [has_uncurry.uncurry],
-  specialize H (g x), 
-  simp only [coe_sort_tt, set.mem_range_self, forall_true_left] at H,
-  revert H, clear hn, generalize : (n (g x)).num_nodes = N, intro H,
-  induction N with N ih,
-  { simp, },
-  rw [iterate_succ_apply', ih (λ m hm, H m $ hm.trans N.le_succ), hf,
-    tree.guard_size_pos, iterate_succ_apply'], { refl, },
-  simpa [has_uncurry.uncurry, iterate_succ'] using H (N + 1) rfl.le,  
-end
-
-/- We now extract `it₃` and `it₄` in the general case unconditionally -/
-theorem iterate {n : α → ℕ} {f : α → β → β} {g : α → β} (hn : n ∈ₑ PTIME)
+theorem iterate [polysize α] [polysize β] {n : α → ℕ} {f : α → β → β} {g : α → β} (hn : n ∈ₑ PTIME)
   (hf : f ∈ₑ PTIME) (hg : g ∈ₑ PTIME) :
   (∃ p : polynomial ℕ, ∀ x (m ≤ n x), size ((f x)^[m] (g x)) ≤ p.eval (size x)) →
   polytime.mem (λ x, (f x)^[n x] (g x))
-| ⟨p, hp⟩ := it₃ (it_all _ _) hn hf hg ⟨polynomial.to_mv 0 p, by simpa using hp⟩
+| ⟨p, hp⟩ :=
+let ⟨q₁, hq₁⟩ := polysize.upper α, ⟨q₂, hq₂⟩ := polysize.lower β in
+ iterate_encode_size hn hf hg ⟨q₂.comp (p.comp q₁),
+ λ x m hm, by { simpa using (hq₂ _).trans (q₂.eval_mono $ (hp x m hm).trans $ p.eval_mono $ hq₁ _), }⟩
 
-theorem iterate_safe_invariant {n : α → ℕ} {f : α → β → β} {g : α → β}
-  (inv : α → β → Prop) (hn : n ∈ₑ PTIME) (hf : f ∈ₑ PTIME) (hg : g ∈ₑ PTIME)
-  (hinv : ∀ x y, inv x y → inv x (f x y)) (h₀ : ∀ x, inv x (g x))
-  (hp : ∃ (p : polynomial ℕ), ∀ x y, inv x y → size (f x y) ≤ size y + p.eval (size x)) :
-  polytime.mem (λ x, (f x)^[n x] (g x)) :=
-let ⟨p', hp'⟩ := polysize_safe.iterate_invariant inv hinv hp (polytime.size_le hn) in 
-it₃ (it_all _ _) hn hf hg ⟨p', λ x m hm y hy, hp' x y m hm ((hy rfl).symm ▸ (h₀ x))⟩
-
-local attribute [-complexity] iterate_safe'
-
-@[complexity] theorem iterate_safe {n : α → ℕ} {f : α → β → β} {g : α → β} (hn : n ∈ₑ PTIME)
+@[complexity] theorem iterate_safe [polysize α] [polysize β] {n : α → ℕ} {f : α → β → β} {g : α → β} (hn : n ∈ₑ PTIME)
   (hf : f ∈ₑ PTIME) (hg : g ∈ₑ PTIME) (hp : polysize_safe f) : polytime.mem (λ x, (f x)^[n x] (g x)) :=
-it₄ (it_all _ _) hn hf hg hp
+let ⟨p₁, hp₁⟩ := polytime.size_le hg, ⟨p₂, hp₂⟩ := polytime.size_le hn in
+iterate hn hf hg ⟨p₁ + p₂ * hp.poly, λ x m hm,
+  (hp.size_le m x (g x)).trans (by { simp, mono*, exacts [hm.trans (hp₂ _), zero_le'], })⟩
 
 end iterate
 
